Sliding window, WIP.

code/Yazi.LZ77.fst
@@ -6,6 +6,10 @@ module Cast = FStar.Int.Cast
 module CB = LowStar.ConstBuffer
 module CFlags = Yazi.CFlags
 module CRC32 = Yazi.CRC32
+module I32 = FStar.Int32
+module LB = Lib.Buffer
+module Math = FStar.Math.Lemmas
+module S = Spec.LZ77
 module ST = FStar.HyperStack.ST
 module U16 = FStar.UInt16
 module U32 = FStar.UInt32
@@ -13,53 +17,62 @@ module U8 = FStar.UInt8
 
 open LowStar.BufferOps
 open FStar.Mul
-open Spec.LZ77
 open Lib.Seq
+open Lib.Buffer
 
-let context_valid (c: lz77_context) =
+type context_p = ctx: CB.const_buffer lz77_context {CB.length ctx == 1}
+
+let context_valid (h: HS.mem) (ctx: context_p) =
   let open U16 in
-  is_window_bits (v c.w_bits) /\
-  is_window_mask (v c.w_bits) (v c.w_mask) /\
-  is_window_size (v c.w_bits) (U32.v c.w_size) /\
-  (U32.v c.window_size) == (U32.v c.w_size) * 2 /\
+  CB.length ctx == 1 /\
+  (let c = B.get h (CB.as_mbuf ctx) 0 in
+  S.is_window_bits (v c.w_bits) /\
+  S.is_window_mask (v c.w_bits) (v c.w_mask) /\
+  S.is_window_size (v c.w_bits) (U32.v c.w_size) /\
+  U32.v c.window_size == (U32.v c.w_size) * 2 /\
   B.length c.window == U32.v c.window_size /\
   B.length c.prev == U32.v c.w_size /\
-  is_hash_bits (v c.h_bits) /\
-  is_hash_size (v c.h_bits) (U32.v c.h_size) /\
-  is_hash_mask (v c.h_bits) (v c.h_mask) /\
-  is_hash_shift (v c.h_bits) (v c.shift) /\
-  B.length c.head == U32.v c.h_size
+  S.is_hash_bits (v c.h_bits) /\
+  S.is_hash_size (v c.h_bits) (U32.v c.h_size) /\
+  S.is_hash_mask (v c.h_bits) (v c.h_mask) /\
+  S.is_hash_shift (v c.h_bits) (v c.shift) /\
+  B.length c.head == U32.v c.h_size /\
+  CB.live h ctx /\ B.live h c.prev /\ B.live h c.window /\ B.live h c.head /\ B.live h c.prev /\
+  B.disjoint c.window c.prev /\ B.disjoint c.window c.head /\ B.disjoint c.prev c.head /\
+  B.frameOf c.window == B.frameOf c.prev /\ B.frameOf c.prev == B.frameOf c.head /\
+  B.frameOf (CB.as_mbuf ctx) <> B.frameOf c.prev /\
+  HS.disjoint (B.frameOf (CB.as_mbuf ctx)) (B.frameOf c.prev))
 
 #set-options "--fuel 0 --ifuel 0"
 inline_for_extraction
 let update_hash
   (a b c: Ghost.erased U8.t)
-  (ctx: CB.const_buffer lz77_context)
+  (ctx: context_p)
   (ins_h: B.pointer U16.t)
   (d: U8.t):
   ST.StackInline unit
   (ensures fun h ->
     let open U16 in
-    CB.length ctx == 1 /\
+    context_valid h ctx /\
+    B.live h ins_h /\ B.disjoint ins_h (CB.as_mbuf ctx) /\
     (let ctx' = B.get h (CB.as_mbuf ctx) 0 in
-    CB.live h ctx /\ B.live h ins_h /\ B.disjoint ins_h (CB.as_mbuf ctx) /\
-    context_valid ctx' /\
-    is_rolling_hash (v ctx'.h_bits) a b c (B.get h ins_h 0)))
+    HS.disjoint (B.frameOf ins_h) (B.frameOf ctx'.head) /\
+    S.is_rolling_hash (v ctx'.h_bits) a b c (B.get h ins_h 0)))
   (requires fun h0 _ h1 ->
     let open U16 in
     let ctx' = B.get h1 (CB.as_mbuf ctx) 0 in
     let hash = B.get h1 ins_h 0 in
     B.modifies (B.loc_buffer ins_h) h0 h1 /\
-    is_rolling_hash (v ctx'.h_bits) b c d (B.get h1 ins_h 0)) =
+    S.is_rolling_hash (v ctx'.h_bits) b c d (B.get h1 ins_h 0)) =
   let open U16 in
   [@inline_let] let d' = Cast.uint8_to_uint16 d in
   let bits = (CB.index ctx 0ul).h_bits in
-  let bits': Ghost.erased hash_bits = Ghost.hide (v bits) in
+  let bits': Ghost.erased S.hash_bits = Ghost.hide (v bits) in
   let s = (CB.index ctx 0ul).shift in
   let m = (CB.index ctx 0ul).h_mask in
   [@inline_let] let s' = Cast.uint16_to_uint32 s in
   let hash = !*ins_h in
-  roll_hash_eq bits' m s a b c d hash;
+  S.roll_hash_eq bits' m s a b c d hash;
   ins_h *= (((hash <<^ s') ^^ d') &^ m)
 
 #set-options "--z3rlimit 200 --fuel 0 --ifuel 0"
@@ -71,7 +84,7 @@ let read_buf ss uncompressed next_in buf size wrap =
   else
     avail_in
   in
-  [@inline_let] let avail_in' = B.sub ss 0ul 1ul in
+  let avail_in' = B.sub ss 0ul 1ul in
   let next_in' = !*next_in in
   let ulen = Ghost.hide (Seq.length uncompressed) in
     
@@ -91,3 +104,193 @@ let read_buf ss uncompressed next_in buf size wrap =
   ss.(1ul) <- U32.add_underspec ss.(1ul) len;
   (len, Ghost.hide buf')
 
+let w_size_fit_u32 (w_size: U32.t{U32.v w_size < pow2 15}): Lemma
+  (ensures 2 * U32.v w_size < pow2 32)
+  [SMTPat (2 * U32.v w_size)] = 
+  Math.pow2_double_mult 15
+
+#set-options "--z3rlimit 2048 --fuel 0 --ifuel 0"
+inline_for_extraction
+let rec slide_head (ctx: context_p) (h_size w_range: Ghost.erased U32.t) (i: U32.t):
+  ST.Stack unit
+  (requires fun h ->
+    let open U32 in
+    context_valid h ctx /\
+    (let ctx' = B.get h (CB.as_mbuf ctx) 0 in
+    U32.v i <= U32.v ctx'.h_size /\
+    U32.v h_size == U32.v ctx'.h_size /\
+    U32.v ctx'.w_size <= U32.v w_range /\ U32.v w_range <= 2 * U32.v ctx'.w_size /\
+    S.sub_head_valid
+      h ctx'.h_bits ctx'.w_size w_range ctx'.h_size
+      (fun j -> j >= U32.v i /\ j < U32.v ctx'.h_size)
+      ctx'.head ctx'.window /\
+    S.sub_head_valid
+      h ctx'.h_bits ctx'.w_size (w_range -^ ctx'.w_size) ctx'.h_size
+      (fun j -> j < U32.v i)
+      ctx'.head (S.slided_window ctx'.w_size w_range ctx'.window)))
+  (ensures fun h0 _ h1 ->
+    let open U32 in
+    context_valid h1 ctx /\
+    (let ctx' = B.get h0 (CB.as_mbuf ctx) 0 in
+    let ctx'' = B.get h1 (CB.as_mbuf ctx) 0 in
+    B.modifies (B.loc_buffer ctx'.head) h0 h1 /\
+    S.head_valid
+      h1 ctx'.h_bits ctx'.w_size (w_range -^ ctx'.w_size) ctx'.h_size
+      ctx'.head (S.slided_window ctx'.w_size w_range ctx'.window)))
+  (decreases U32.v h_size - U32.v i) =
+  let open U32 in
+  let head = (CB.index ctx 0ul).head in
+  let w_size = (CB.index ctx 0ul).w_size in
+  if i <^ (CB.index ctx 0ul).h_size then begin
+    let m = head.(i) in
+    [@inline_let] let m' = Cast.uint16_to_uint32 m in
+    head.(i) <- Cast.uint32_to_uint16 (if m' >=^ w_size then m' -^ w_size else 0ul);
+    slide_head ctx h_size w_range (i +^ 1ul)
+  end else
+    ()
+
+inline_for_extraction
+let rec slide_prev (ctx: context_p) (w_size w_range: Ghost.erased U32.t) (i: U32.t):
+  ST.Stack unit
+  (requires fun h ->
+    let open U32 in
+    context_valid h ctx /\
+    (let ctx' = B.get h (CB.as_mbuf ctx) 0 in
+    CFlags.fastest == false /\
+    U32.v i <= U32.v ctx'.w_size /\
+    U32.v w_size == U32.v ctx'.w_size /\
+    U32.v ctx'.w_size <= U32.v w_range /\ U32.v w_range <= 2 * U32.v ctx'.w_size /\
+    S.sub_prev_valid h
+      ctx'.w_bits ctx'.w_size
+      (fun j -> v i <= j /\ j < v w_size)
+      ctx'.prev (B.gsub ctx'.window 0ul w_range) /\
+    S.sub_prev_valid h
+      ctx'.w_bits ctx'.w_size
+      (fun j -> j < v i)
+      ctx'.prev (S.slided_window ctx'.w_size w_range ctx'.window)))
+  (ensures fun h0 _ h1 ->
+    context_valid h1 ctx /\
+    (let ctx' = B.get h1 (CB.as_mbuf ctx) 0 in
+    B.modifies (B.loc_buffer ctx'.prev) h0 h1 /\
+    S.prev_valid h1
+      ctx'.w_bits ctx'.w_size
+      ctx'.prev (S.slided_window ctx'.w_size w_range ctx'.window)))
+  (decreases U32.v w_size - U32.v i) =
+  let open U32 in
+  let prev = (CB.index ctx 0ul).prev in
+  let w_size' = (CB.index ctx 0ul).w_size in
+  if i <^ w_size' then begin
+    let m = prev.(i) in
+    [@inline_let] let m' = Cast.uint16_to_uint32 m in
+    prev.(i) <- Cast.uint32_to_uint16 (if m' >=^ w_size' then m' -^ w_size' else 0ul);
+    slide_prev ctx w_size w_range (i +^ 1ul)
+  end else
+    ()
+
+inline_for_extraction
+let slide_window_buf
+  (ctx: context_p)
+  (state: lz77_state)
+  (block_start: B.pointer I32.t)
+  (len: U32.t):
+  ST.Stack unit
+  (requires fun h ->
+    let open U32 in
+    context_valid h ctx /\
+    (let ctx' = B.get h (CB.as_mbuf ctx) 0 in
+    v len <= v ctx'.w_size /\
+    S.slide_window_pre h ctx'.w_bits state block_start ctx'.w_size ctx'.window))
+  (ensures fun h0 _ h1 -> 
+    context_valid h0 ctx /\
+    (let ctx' = B.get h0 (CB.as_mbuf ctx) 0 in
+    B.modifies (
+      B.loc_buffer block_start `B.loc_union`
+      B.loc_buffer state `B.loc_union`
+      B.loc_buffer ctx'.window) h0 h1 /\
+    S.slide_window_buf_post h0 h1
+      ctx'.w_bits state block_start ctx'.w_size ctx'.window len)) =
+  let open U32 in
+  let w_size = (CB.index ctx 0ul).w_size in
+  let window = (CB.index ctx 0ul).window in
+  let w_bits = Ghost.hide (CB.index ctx 0ul).w_bits in
+  S.window_size_upper_bound (U16.v w_bits) (v w_size);
+  let left = B.sub window 0ul w_size in
+  let right = B.sub window w_size w_size in
+  B.blit right 0ul left 0ul len;
+  set_match_start (U16.v w_bits) (v w_size) state ((get_match_start state) -^ w_size);
+  set_strstart (U16.v w_bits) (v w_size) state ((get_strstart state) -^ w_size);
+  block_start *= I32.sub (!*block_start) (Cast.uint32_to_int32 w_size)
+
+#set-options "--z3rlimit 4096 --fuel 0 --ifuel 0"
+inline_for_extraction
+let slide_window
+  (ctx: context_p)
+  (state: lz77_state)
+  (block_start: B.pointer I32.t):
+  ST.Stack U32.t
+  (requires fun h ->
+    let open U32 in
+    let ctx' = B.get h (CB.as_mbuf ctx) 0 in
+    let state' = B.as_seq h state in
+    context_valid h ctx /\
+    B.disjoint (CB.as_mbuf ctx) state /\ B.disjoint (CB.as_mbuf ctx) block_start /\
+    HS.disjoint (B.frameOf state) (B.frameOf ctx'.head) /\
+    HS.disjoint (B.frameOf block_start) (B.frameOf ctx'.head) /\
+
+    S.slide_window_pre h ctx'.w_bits state block_start ctx'.w_size ctx'.window /\
+    (let w_range = U32.uint_to_t (S.strstart state' - S.insert state') in
+    S.hash_chain_valid h
+      ctx'.w_bits ctx'.h_bits
+      ctx'.w_size ctx'.h_size
+      ctx'.head ctx'.prev (B.gsub ctx'.window 0ul w_range)
+      w_range))
+  (ensures fun h0 more h1 ->
+    let open U32 in
+    let ctx' = B.get h0 (CB.as_mbuf ctx) 0 in
+    let ctx1 = B.get h1 (CB.as_mbuf ctx) 0 in
+    let s0 = B.as_seq h0 state in
+    let s1 = B.as_seq h1 state in
+    S.slided_window_space_valid s0 ctx'.w_size more /\
+    (S.strstart s0 < U32.v ctx'.w_size ==> B.modifies B.loc_none h0 h1) /\
+    (S.strstart s0 >= U32.v ctx'.w_size ==>
+      S.lookahead s1 + S.strstart s1 <= U32.v ctx'.w_size /\
+      (let len = uint_to_t (S.lookahead s1 + S.strstart s1) in
+      B.modifies (
+        B.loc_buffer block_start `B.loc_union`
+        B.loc_buffer state `B.loc_union`
+        B.loc_buffer ctx'.window `B.loc_union`
+        B.loc_buffer ctx'.head `B.loc_union`
+        (if CFlags.fastest then B.loc_none else B.loc_buffer ctx'.prev)) h0 h1 /\
+      S.slide_window_buf_post h0 h1
+        ctx'.w_bits state block_start
+        ctx'.w_size ctx'.window len /\
+      (let w_range = uint_to_t (S.strstart s1 - S.insert s1) in
+      B.as_seq h0 (B.gsub ctx'.window ctx'.w_size w_range) ==
+      B.as_seq h1 (B.gsub ctx'.window 0ul w_range) /\
+      S.hash_chain_valid h1
+        ctx'.w_bits ctx'.h_bits
+        ctx'.w_size ctx'.h_size
+        ctx'.head ctx'.prev ctx'.window
+        w_range
+      )))) =
+  let h0 = Ghost.hide (ST.get ()) in
+  let open U32 in
+  let strstart = get_strstart state in
+  let w_size = (CB.index ctx 0ul).w_size in
+  let w_bits = Ghost.hide (CB.index ctx 0ul).w_bits in
+  let w_range = Ghost.hide (strstart -^ get_insert state) in
+  let h_size = Ghost.hide (CB.index ctx 0ul).h_size in
+  let h_bits = Ghost.hide (CB.index ctx 0ul).h_bits in
+  let window = Ghost.hide (CB.index ctx 0ul).window in
+  let head = Ghost.hide (CB.index ctx 0ul).head in
+  let more = (CB.index ctx 0ul).window_size -^ get_lookahead state -^ strstart in
+  if strstart >=^ w_size then begin
+    slide_head ctx h_size w_range 0ul;
+    if CFlags.fastest then () else slide_prev ctx w_size w_range 0ul;
+    slide_window_buf ctx state block_start (w_size -^ more);
+
+    let h1 = Ghost.hide (ST.get ()) in
+    LB.as_seq_gsub_eq h0 h1 window window w_size 0ul (w_size -^ more) (w_range -^ w_size);
+    more +^ w_size
+  end else
+    more
