code/Yazi.LZ77.fsti
@@ -6,7 +6,7 @@ module CFlags = Yazi.CFlags
 module CRC32 = Spec.CRC32
 module HS = FStar.HyperStack
 module I32 = FStar.Int32
-module S = Spec.State
+module SS = Spec.Stream
 module Seq = FStar.Seq
 module ST = FStar.HyperStack.ST
 module U16 = FStar.UInt16
@@ -14,17 +14,19 @@ module U32 = FStar.UInt32
 module U8 = FStar.UInt8
 module Util = Yazi.Util
 
+include Yazi.LZ77.State
+
 noeq type lz77_context = {
-  w_size: U32.t;        (* LZ77 window size (32K by default) *)
-  w_bits: U16.t;        (* log2 w_size  (8..16) *)
-  w_mask: U16.t;        (* w_size - 1 *)
+  w_size: U32.t; (* LZ77 window size (32K by default) *)
+  w_bits: U16.t; (* log2 w_size  (8..16) *)
+  w_mask: U16.t; (* w_size - 1 *)
 
   (* Sliding window. Input bytes are read into the second half of the window,
    * and move to the first half later to keep a dictionary of at least wSize
    * bytes. With this organization, matches are limited to a distance of
    * wSize-MAX_MATCH bytes, but this ensures that IO is always
    * performed with a length multiple of the block size. Also, it limits
-   * the window size to 64K, which is quite useful on MSDOS.
+   * the window size to 64K.
    * To do: use the user input buffer as sliding window. *)
   window: B.buffer U8.t;
 
@@ -50,24 +52,6 @@ noeq type lz77_context = {
   shift: U16.t;
 }
 
-noeq type lz77_state = {
-  (* Window position at the beginning of the current output block. Gets
-   * negative when the window is moved backwards. *)
-  block_start: I32.t;
-
-  ins_h: U32.t;        (* hash index of string to be inserted *)
-  match_length: U32.t; (* length of best match *)
-  prev_match: U32.t;   (* previous match *)
-  strstart: U32.t;     (* start of string to insert *)
-  match_start: U32.t;  (* start of matching string *)
-  lookahead: U32.t;    (* number of valid bytes ahead in window *)
-
-  (* Length of the best match at previous step. Matches not greater than this
-   * are discarded. This is used in the lazy match evaluation. *)
-  prev_length: U32.t;
-  match_available: bool; (* set if previous match exists *)
-}
-
 type stream_state = B.lbuffer U32.t 5
 
 val read_buf:
@@ -79,8 +63,8 @@ val read_buf:
   -> wrap: I32.t
   -> ST.Stack (U32.t & Ghost.erased (B.buffer U8.t))
   (requires fun h -> 
-    let len = if U32.v size > S.avail_in (B.as_seq h ss) then
-      S.avail_in (B.as_seq h ss)
+    let len = if U32.v size > SS.avail_in (B.as_seq h ss) then
+      SS.avail_in (B.as_seq h ss)
     else
       U32.v size
     in
@@ -89,16 +73,16 @@ val read_buf:
     B.live h buf /\ ~(B.g_is_null buf) /\
     HS.disjoint (B.frameOf ss) (B.frameOf buf) /\
     B.length buf == U32.v size /\
-    S.next_in_valid h ss next_in /\
-    S.adler_valid h ss wrap uncompressed)
+    SS.next_in_valid h ss next_in /\
+    SS.adler_valid h ss wrap uncompressed)
   (ensures fun h0 res h1 ->
   let (len', read) = res in
   let next_in0 = B.get h0 next_in 0 in
   let next_in1 = B.get h1 next_in 0 in
   let s0 = B.as_seq h0 ss in
   let s1 = B.as_seq h1 ss in
-  let len = if U32.v size > S.avail_in s0 then
-    S.avail_in s0
+  let len = if U32.v size > SS.avail_in s0 then
+    SS.avail_in s0
   else
     U32.v size
   in
@@ -107,8 +91,8 @@ val read_buf:
     (B.loc_buffer ss)
     (B.loc_union (B.loc_buffer next_in) (B.loc_buffer buf))) h0 h1 /\
   Seq.equal (B.as_seq h1 read) (B.as_seq h0 (B.gsub next_in0 0ul len')) /\
-  S.avail_in s0 - len == S.avail_in s1 /\
-  S.next_in_valid h1 ss next_in /\
-  S.adler_valid h1 ss wrap (Seq.append uncompressed (B.as_seq h1 read)) /\
-  S.avail_out s0 == S.avail_out s1 /\
-  S.total_out s0 == S.total_out s1)
+  SS.avail_in s0 - len == SS.avail_in s1 /\
+  SS.next_in_valid h1 ss next_in /\
+  SS.adler_valid h1 ss wrap (Seq.append uncompressed (B.as_seq h1 read)) /\
+  SS.avail_out s0 == SS.avail_out s1 /\
+  SS.total_out s0 == SS.total_out s1)
