lib/Lib.Buffer.fsti
@@ -3,6 +3,9 @@ module Lib.Buffer
 module B = LowStar.Buffer
 module HS = FStar.HyperStack
 module Seq = FStar.Seq
+module U32 = FStar.UInt32
+
+open Lib.Seq
 
 let append_empty_buf_r (#a: Type) (h: HS.mem) (buf: B.buffer a) (s: Seq.seq a): Lemma
   (requires B.length buf == 0)
@@ -12,3 +15,29 @@ let append_empty_buf_r (#a: Type) (h: HS.mem) (buf: B.buffer a) (s: Seq.seq a): 
   Seq.lemma_empty (B.as_seq h buf);
   Seq.append_empty_r s
 
+let unchange_except
+  (#a: Type)
+  (h0 h1: HS.mem)
+  (buf: B.buffer a)
+  (i: nat{i < B.length buf}) =
+  let s0 = B.as_seq h0 buf in
+  let s1 = B.as_seq h1 buf in
+  forall (j: nat{j < B.length buf /\ j <> i}). Seq.index s0 j == Seq.index s1 j
+
+let as_seq_gsub_eq
+  (#a: Type)
+  (h0 h1: HS.mem)
+  (b0 b1: B.buffer a)
+  (s0 s1 l l': U32.t): Lemma
+  (requires
+    U32.v s0 + U32.v l <= B.length b0 /\ U32.v s1 + U32.v l <= B.length b1 /\
+    B.as_seq h0 (B.gsub b0 s0 l) == B.as_seq h1 (B.gsub b1 s1 l) /\
+    U32.v l' <= U32.v l)
+  (ensures B.as_seq h0 (B.gsub b0 s0 l') == B.as_seq h1 (B.gsub b1 s1 l')) =
+  let sq0 = B.as_seq h0 (B.gsub b0 s0 l) in
+  let sq1 = B.as_seq h1 (B.gsub b1 s1 l) in
+  let sq0' = Seq.slice (B.as_seq h0 b0) (U32.v s0) (U32.v l' + U32.v s0) in
+  let sq1' = Seq.slice (B.as_seq h1 b1) (U32.v s1) (U32.v l' + U32.v s1) in
+  assert(forall (i: nat{i < U32.v l'}).
+    sq0.[i] == sq0'.[i] /\ sq1.[i] == sq1'.[i] /\ sq0.[i] == sq1.[i]);
+  assert(Seq.equal sq0' sq1')
