specs/Spec.LZ77.fsti
@@ -1,14 +1,22 @@
 module Spec.LZ77
 
+module B = LowStar.Buffer
 module Cast = FStar.Int.Cast
+module CFlags = Yazi.CFlags
+module HS = FStar.HyperStack
+module I32 = FStar.Int32
+module Math = FStar.Math.Lemmas
 module U8 = FStar.UInt8
 module U16 = FStar.UInt16
+module U32 = FStar.UInt32
 
 open FStar.Mul
 open Lib.UInt
+open Lib.Seq
 
 let min_match = 3
 let max_match = 258
+let min_lookhead = max_match + min_match + 1
 
 unfold let is_hash_bits (b: nat) = b >= 8 /\ b <= 16
 type hash_bits = b: nat{is_hash_bits b}
@@ -30,6 +38,9 @@ type window_mask (bits: window_bits) = m: nat{is_window_mask bits m}
 
 unfold let is_window_size (b: window_bits) (s: nat) = s == pow2 b
 type window_size (bits: window_bits) = s: nat{is_window_size bits s}
+
+let window_size_upper_bound (b: window_bits) (w_size: window_size b): Lemma
+  (ensures w_size <= 32768) = assert_norm(w_size == pow2 b)
 
 #set-options "--z3rlimit 120 --fuel 8 --ifuel 8"
 let is_rolling_hash (bits: hash_bits) (a b c: U8.t) (h: U16.t) =
@@ -62,3 +73,165 @@ val roll_hash_eq:
   (ensures is_rolling_hash bits b c d (
     U16.logand (U16.logxor (U16.shift_left h (Cast.uint16_to_uint32 shift)) (Cast.uint8_to_uint16 d)) mask
   ))
+
+unfold let slided_window
+  (w_size: U32.t)
+  (w_range: U32.t{U32.v w_size <= U32.v w_range /\ U32.v w_range <= 2 * U32.v w_size})
+  (window: B.lbuffer U8.t (2 * U32.v w_size)) =
+  let open U32 in
+  B.gsub window w_size (w_range -^ w_size)
+  
+unfold let sub_head_valid
+  (h: HS.mem)
+  (h_bits: U16.t {is_hash_bits (U16.v h_bits)})
+  (w_size: U32.t)
+  (w_range: U32.t{U32.v w_range <= 2 * U32.v w_size})
+  (h_size: U32.t{is_hash_size (U16.v h_bits) (U32.v h_size)})
+  (range: (i: nat) -> (p:Type0{p ==> i < U32.v h_size}))
+  (head: B.lbuffer U16.t (U32.v h_size))
+  (window: B.buffer U8.t{B.length window >= U32.v w_range}) =
+  let open U32 in
+  let head' = B.as_seq h head in
+  let window' = B.as_seq h window in
+  B.live h head /\ B.live h window /\ B.disjoint head window /\
+  (forall (i: nat{range i /\ U16.v head'.[i] <> 0}).
+    U16.v head'.[i] <= v w_range - min_match /\
+    is_rolling_hash
+      (U16.v h_bits)
+      window'.[U16.v head'.[i]]
+      window'.[1 + U16.v head'.[i]]
+      window'.[2 + U16.v head'.[i]]
+      (U16.uint_to_t i))
+  
+unfold let head_valid
+  (h: HS.mem)
+  (h_bits: U16.t {is_hash_bits (U16.v h_bits)})
+  (w_size: U32.t)
+  (w_range: U32.t{U32.v w_range <= 2 * U32.v w_size})
+  (h_size: U32.t{is_hash_size (U16.v h_bits) (U32.v h_size)})
+  (head: B.lbuffer U16.t (U32.v h_size))
+  (window: B.buffer U8.t{B.length window >= U32.v w_range}) =
+  sub_head_valid
+    h h_bits w_size w_range h_size
+    (fun j -> j < U32.v h_size)
+    head window
+
+#set-options "--z3rlimit 120 --fuel 0 --ifuel 0"
+let sub_prev_valid
+  (h: HS.mem)
+  (w_bits: U16.t {is_window_bits (U16.v w_bits)})
+  (w_size: U32.t{is_window_size (U16.v w_bits) (U32.v w_size)})
+  (range: (i: nat) -> (p: Type0{p ==> i < U32.v w_size}))
+  (prev: B.lbuffer U16.t (U32.v w_size))
+  (window: B.buffer U8.t{B.length window <= 2 * U32.v w_size}) =
+  let open Lib.Seq in
+  let prev' = B.as_seq h prev in
+  let window' = B.as_seq h window in
+  B.live h prev /\ B.live h window /\ B.disjoint prev window /\
+  (forall (i: nat{i < B.length window}).
+    let j = i % U32.v w_size in
+    Math.lemma_mod_lt i (U32.v w_size);
+    range j ==>
+      (U16.v prev'.[j] < i /\
+      (U16.v prev'.[j] <> 0 ==> window'.[U16.v prev'.[j]] == window'.[j])))
+
+unfold let prev_valid
+  (h: HS.mem)
+  (w_bits: U16.t {is_window_bits (U16.v w_bits)})
+  (w_size: U32.t{is_window_size (U16.v w_bits) (U32.v w_size)})
+  (prev: B.lbuffer U16.t (U32.v w_size))
+  (window: B.buffer U8.t{B.length window <= 2 * U32.v w_size}) =
+  sub_prev_valid h w_bits w_size (fun j -> j < U32.v w_size) prev window
+
+unfold let hash_chain_valid
+  (h: HS.mem)
+  (w_bits: U16.t {is_window_bits (U16.v w_bits)})
+  (h_bits: U16.t {is_hash_bits (U16.v h_bits)})
+  (w_size: U32.t{is_window_size (U16.v w_bits) (U32.v w_size)})
+  (h_size: U32.t{is_hash_size (U16.v h_bits) (U32.v h_size)})
+  (head: B.lbuffer U16.t (U32.v h_size))
+  (prev: B.lbuffer U16.t (U32.v w_size))
+  (window: B.buffer U8.t)
+  (w_range: U32.t{U32.v w_range <= 2 * U32.v w_size}) =
+  B.length window >= U32.v w_range /\
+  (CFlags.fastest == false ==>
+    prev_valid h w_bits w_size prev (B.gsub window 0ul w_range)) /\
+  head_valid h h_bits w_size w_range h_size head (B.gsub window 0ul w_range)
+
+type lz77_state = s:Seq.seq U32.t{Seq.length s == 8}
+
+open Lib.Seq
+
+unfold let ins_h (s: lz77_state) = U32.v s.[0]
+unfold let match_length (s: lz77_state) = U32.v s.[1]
+unfold let match_start (s: lz77_state) = U32.v s.[2]
+unfold let prev_match (s: lz77_state) = U32.v s.[3]
+unfold let prev_length (s: lz77_state) = U32.v s.[4]
+unfold let strstart (s: lz77_state) = U32.v s.[5]
+unfold let lookahead (s: lz77_state) = U32.v s.[6]
+unfold let insert (s: lz77_state) = U32.v s.[7]
+
+unfold let ins_h_unchange (s0 s1: lz77_state) = ins_h s0 == ins_h s1
+unfold let match_length_unchange (s0 s1: lz77_state) = match_length s0 == match_length s1
+unfold let match_start_unchange (s0 s1: lz77_state) = match_start s0 == match_start s1
+unfold let prev_match_unchange (s0 s1: lz77_state) = prev_match s0 == prev_match s1
+unfold let prev_length_unchange (s0 s1: lz77_state) = prev_length s0 == prev_length s1
+unfold let strstart_unchange (s0 s1: lz77_state) = strstart s0 == strstart s1
+unfold let lookahead_unchange (s0 s1: lz77_state) = lookahead s0 == lookahead s1
+unfold let insert_unchange (s0 s1: lz77_state) = insert s0 == insert s1
+
+let strstart_lookahead_valid
+  (s: lz77_state)
+  (w_bits: U16.t{is_window_bits (U16.v w_bits)})
+  (w_size: U32.t{is_window_size (U16.v w_bits) (U32.v w_size)}) =
+  strstart s + lookahead s <= 2 * U32.v w_size
+
+unfold let slided_window_space_valid (s: lz77_state) (w_size more: U32.t) =
+  let open U32 in
+  (strstart s >= v w_size ==>
+    v more == 2 * v w_size - lookahead s - strstart s + v w_size) /\
+  (strstart s < v w_size ==>
+    v more == 2 * v w_size - lookahead s - strstart s)
+
+// TODO: verify block_start's lower bound
+unfold let slide_window_pre
+  (h: HS.mem)
+  (w_bits: U16.t {is_window_bits (U16.v w_bits)})
+  (state: B.lbuffer U32.t 8)
+  (block_start: B.pointer I32.t)
+  (w_size: U32.t{is_window_size (U16.v w_bits) (U32.v w_size)})
+  (window: B.lbuffer U8.t (2 * U32.v w_size)) =
+  let open U32 in
+  let state' = B.as_seq h state in
+  B.live h block_start /\ B.live h window /\ B.live h state /\
+  B.disjoint state window /\ B.disjoint state block_start /\ B.disjoint window block_start /\
+  match_start state' >= v w_size /\
+  match_start state' < 2 * v w_size /\
+  strstart state' >= v w_size /\
+  strstart state' < 2 * v w_size /\
+  insert state' <= strstart state' - v w_size /\
+  strstart_lookahead_valid state' w_bits w_size /\
+  I32.v (B.get h block_start 0) >= -8454144
+
+unfold let slide_window_buf_post
+  (h0 h1: HS.mem)
+  (w_bits: U16.t{is_window_bits (U16.v w_bits)})
+  (state: B.lbuffer U32.t 8)
+  (block_start: B.pointer I32.t)
+  (w_size: U32.t{is_window_size (U16.v w_bits) (U32.v w_size)})
+  (window: B.lbuffer U8.t (2 * U32.v w_size))
+  (len: U32.t{U32.v len <= U32.v w_size}) =
+  let s0 = B.as_seq h0 state in
+  let s1 = B.as_seq h1 state in
+  let w0 = B.as_seq h0 window in
+  let w1 = B.as_seq h1 window in
+  let w_size' = U32.v w_size in
+  ins_h_unchange s0 s1 /\ match_length_unchange s0 s1 /\
+  prev_match_unchange s0 s1 /\ prev_length_unchange s0 s1 /\
+  lookahead_unchange s0 s1 /\ insert_unchange s0 s1 /\
+  strstart s0 - U32.v w_size == strstart s1 /\
+  match_start s0 - U32.v w_size == match_start s1 /\
+  strstart_lookahead_valid s1 w_bits w_size /\
+  I32.v (B.get h0 block_start 0) - U32.v w_size == I32.v (B.get h1 block_start 0) /\
+  Seq.slice w0 w_size' (w_size' + U32.v len) == Seq.slice w1 0 (U32.v len) /\
+  B.as_seq h0 (B.gsub window w_size len) == B.as_seq h1 (B.gsub window 0ul len)
