code/Yazi.LZ77.State.fst
@@ -1,0 +1,76 @@
+module Yazi.LZ77.State
+
+module B = LowStar.Buffer
+module LB = Lib.Buffer
+module S = Spec.LZ77
+module ST = FStar.HyperStack.ST
+module U32 = FStar.UInt32
+
+open FStar.Mul
+open LowStar.BufferOps
+
+type lz77_state = B.lbuffer U32.t 8
+
+inline_for_extraction
+let set_match_start
+  (bits: Ghost.erased S.window_bits)
+  (w_size: Ghost.erased (S.window_size bits))
+  (state: lz77_state)
+  (match_start: U32.t{U32.v match_start < 2 * w_size}):
+  ST.Stack unit
+  (ensures fun h -> B.live h state)
+  (requires fun h0 _ h1 ->
+    B.modifies (B.loc_buffer state) h0 h1 /\
+    S.match_start (B.as_seq h1 state) == U32.v match_start /\
+    LB.unchange_except h0 h1 state 2) =
+  state.(2ul) <- match_start
+
+inline_for_extraction
+let get_match_start (state: lz77_state):
+  ST.Stack U32.t
+  (ensures fun h -> B.live h state)
+  (requires fun h0 res h1 ->
+    B.modifies B.loc_none h0 h1 /\
+    S.match_start (B.as_seq h0 state) == U32.v res) =
+  state.(2ul)
+
+inline_for_extraction
+let set_strstart
+  (bits: Ghost.erased S.window_bits)
+  (w_size: Ghost.erased (S.window_size bits))
+  (state: lz77_state)
+  (strstart: U32.t{U32.v strstart < 2 * w_size}):
+  ST.Stack unit
+  (ensures fun h -> B.live h state)
+  (requires fun h0 _ h1 ->
+    B.modifies (B.loc_buffer state) h0 h1 /\
+    S.strstart (B.as_seq h1 state) == U32.v strstart /\
+    LB.unchange_except h0 h1 state 5) =
+  state.(5ul) <- strstart
+
+inline_for_extraction
+let get_strstart (state: lz77_state):
+  ST.Stack U32.t
+  (ensures fun h -> B.live h state)
+  (requires fun h0 res h1 ->
+    B.modifies B.loc_none h0 h1 /\
+    S.strstart (B.as_seq h0 state) == U32.v res) =
+  state.(5ul)
+
+inline_for_extraction
+let get_lookahead (state: lz77_state):
+  ST.Stack U32.t
+  (ensures fun h -> B.live h state)
+  (requires fun h0 res h1 ->
+    B.modifies B.loc_none h0 h1 /\
+    S.lookahead (B.as_seq h0 state) == U32.v res) =
+  state.(6ul)
+
+inline_for_extraction
+let get_insert (state: lz77_state):
+  ST.Stack U32.t
+  (ensures fun h -> B.live h state)
+  (requires fun h0 res h1 ->
+    B.modifies B.loc_none h0 h1 /\
+    S.insert (B.as_seq h0 state) == U32.v res) =
+  state.(7ul)
